Inductive.v
@@ -1,0 +1,478 @@
+Section Ind1.
+
+Context {A : Type}.
+Context (G : (A -> Prop) -> (A -> Prop)).
+Context (P : A -> Prop).
+
+Implicit Types Q R : A -> Prop.
+
+Definition is_ind1 :=
+  (forall Q R, (forall x, Q x -> R x) -> forall x, G Q x -> G R x) /\ (forall Q, (forall x, G Q x -> Q x) -> forall x, P x -> Q x) /\ (forall x, G P x -> P x).
+
+Hypothesis Hind : is_ind1.
+
+Let is_positive := proj1 Hind.
+Let has_ind := proj1 (proj2 Hind).
+Let is_ind := proj2 (proj2 Hind).
+
+Definition preserved1 Q :=
+  forall x, G (fun x => P x /\ Q x) x -> Q x.
+Definition preserved_with_inv1 Q R :=
+  forall x, G (fun x => P x /\ Q x /\ R x) x -> Q x.
+Definition preserved_down1 Q :=
+  forall x R, G (fun x => P x /\ R x) x -> Q x -> G (fun x => P x /\ Q x /\ R x) x.
+
+Lemma preserved1_rec :
+  forall Q, preserved1 Q -> forall x, P x -> Q x.
+Proof.
+  intros Q HQ.
+  enough (H : forall x, P x -> P x /\ Q x) by (intros; apply H; assumption).
+  apply has_ind. intros; split.
+  - eapply is_ind, is_positive; [|eassumption].
+    simpl. intros; tauto.
+  - apply HQ. assumption.
+Qed.
+
+Lemma preserved_with_inv1_rec :
+  forall Q R, preserved_down1 R -> preserved_with_inv1 Q R -> forall x, P x -> R x -> Q x.
+Proof.
+  intros Q R H1 H2. refine (preserved1_rec (fun x => R x -> Q x) _).
+  intros x H3 H4. apply H2.
+  apply is_positive with (Q := fun x => P x /\ R x /\ (R x -> Q x)); [intros; tauto|].
+  apply H1; assumption.
+Qed.
+
+Lemma ind1_inv :
+  forall x, P x -> G P x.
+Proof.
+  apply preserved1_rec. intros x H.
+  eapply is_positive; [|eassumption].
+  simpl. intros; tauto.
+Qed.
+
+Ltac prove_ind1 :=
+  unfold is_ind1;
+  match goal with [ |- ?G1_ /\ ?G2_ /\ ?G3_ ] =>
+    pose (G1 := G1_);
+    pose (Hmap := (ltac:(intros Q R H x Hx; destruct Hx; constructor; try assumption; apply H; assumption) : G1));
+    split; [exact Hmap|];
+    split; [|intros x Hx; constructor; assumption];
+    intros Q HQ; fix H 2; intros x Hx;
+    destruct Hx as [x1 Hx];
+    apply (Hmap _ Q) in Hx; [apply HQ; assumption|assumption]
+  end.
+
+End Ind1.
+
+Section Ind2.
+
+Context {A : Type}.
+Context {B : A -> Type}.
+Context (G : (forall x, B x -> Prop) -> (forall x, B x -> Prop)).
+Context (P : forall x, B x -> Prop).
+
+Implicit Types Q R : forall x, B x -> Prop.
+
+Definition is_ind2 :=
+  (forall Q R, (forall x y, Q x y -> R x y) -> forall x y, G Q x y -> G R x y) /\
+  (forall Q, (forall x y, G Q x y -> Q x y) -> forall x y, P x y -> Q x y) /\
+  (forall x y, G P x y -> P x y).
+
+Hypothesis Hind : is_ind2.
+
+Let is_positive := proj1 Hind.
+Let has_ind := proj1 (proj2 Hind).
+Let is_ind := proj2 (proj2 Hind).
+
+Definition preserved2 Q :=
+  forall x y, G (fun x y => P x y /\ Q x y) x y -> Q x y.
+Definition preserved_with_inv2 Q R :=
+  forall x y, G (fun x y => P x y /\ Q x y /\ R x y) x y -> Q x y.
+Definition preserved_down2 Q :=
+  forall x y R, G (fun x y => P x y /\ R x y) x y -> Q x y -> G (fun x y => P x y /\ Q x y /\ R x y) x y.
+
+Lemma preserved2_rec :
+  forall Q, preserved2 Q -> forall x y, P x y -> Q x y.
+Proof.
+  intros Q HQ.
+  enough (H : forall x y, P x y -> P x y /\ Q x y) by (intros; apply H; assumption).
+  apply has_ind. intros; split.
+  - eapply is_ind, is_positive; [|eassumption].
+    simpl. intros; tauto.
+  - apply HQ. assumption.
+Qed.
+
+Lemma preserved_with_inv2_rec :
+  forall Q R, preserved_down2 R -> preserved_with_inv2 Q R -> forall x y, P x y -> R x y -> Q x y.
+Proof.
+  intros Q R H1 H2. refine (preserved2_rec (fun x y => R x y -> Q x y) _).
+  intros x y H3 H4. apply H2.
+  apply is_positive with (Q := fun x y => P x y /\ R x y /\ (R x y -> Q x y)); [intros; tauto|].
+  apply H1; assumption.
+Qed.
+
+Lemma ind2_inv :
+  forall x y, P x y -> G P x y.
+Proof.
+  apply preserved2_rec. intros x y H.
+  eapply is_positive; [|eassumption].
+  simpl. intros; tauto.
+Qed.
+
+Ltac prove_ind2 :=
+  unfold is_ind2;
+  match goal with [ |- ?G1_ /\ ?G2_ /\ ?G3_ ] =>
+    pose (G1 := G1_);
+    pose (Hmap := (ltac:(intros Q R H x y Hxy; destruct Hxy; constructor; try assumption; apply H; assumption) : G1));
+    split; [exact Hmap|];
+    split; [|intros x y Hxy; constructor; assumption];
+    intros Q HQ; fix H 3; intros x y Hxy;
+    destruct Hxy as [x1 y1 Hxy];
+    apply (Hmap _ Q) in Hxy; [apply HQ; assumption|assumption]
+  end.
+
+End Ind2.
+
+
+Section Ind3.
+
+Context {A : Type}.
+Context {B : A -> Type}.
+Context {C : forall x, B x -> Type}.
+Context (G : (forall x y, C x y -> Prop) -> (forall x y, C x y -> Prop)).
+Context (P : forall x y, C x y -> Prop).
+
+Implicit Types Q R : forall x y, C x y -> Prop.
+
+Definition is_ind3 :=
+  (forall Q R, (forall x y z, Q x y z -> R x y z) -> forall x y z, G Q x y z -> G R x y z) /\
+  (forall Q, (forall x y z, G Q x y z -> Q x y z) -> forall x y z, P x y z -> Q x y z) /\
+  (forall x y z, G P x y z -> P x y z).
+
+Hypothesis Hind : is_ind3.
+
+Let is_positive := proj1 Hind.
+Let has_ind := proj1 (proj2 Hind).
+Let is_ind := proj2 (proj2 Hind).
+
+Definition preserved3 Q :=
+  forall x y z, G (fun x y z => P x y z /\ Q x y z) x y z -> Q x y z.
+Definition preserved_with_inv3 Q R :=
+  forall x y z, G (fun x y z => P x y z /\ Q x y z /\ R x y z) x y z -> Q x y z.
+Definition preserved_down3 Q :=
+  forall x y z R, G (fun x y z => P x y z /\ R x y z) x y z -> Q x y z -> G (fun x y z => P x y z /\ Q x y z /\ R x y z) x y z.
+
+Lemma preserved3_rec :
+  forall Q, preserved3 Q -> forall x y z, P x y z -> Q x y z.
+Proof.
+  intros Q HQ.
+  enough (H : forall x y z, P x y z -> P x y z /\ Q x y z) by (intros; apply H; assumption).
+  apply has_ind. intros; split.
+  - eapply is_ind, is_positive; [|eassumption].
+    simpl. intros; tauto.
+  - apply HQ. assumption.
+Qed.
+
+Lemma preserved_with_inv3_rec :
+  forall Q R, preserved_down3 R -> preserved_with_inv3 Q R -> forall x y z, P x y z -> R x y z -> Q x y z.
+Proof.
+  intros Q R H1 H2. refine (preserved3_rec (fun x y z => R x y z -> Q x y z) _).
+  intros x y z H3 H4. apply H2.
+  apply is_positive with (Q := fun x y z => P x y z /\ R x y z /\ (R x y z -> Q x y z)); [intros; tauto|].
+  apply H1; assumption.
+Qed.
+
+Lemma ind3_inv :
+  forall x y z, P x y z -> G P x y z.
+Proof.
+  apply preserved3_rec. intros x y z H.
+  eapply is_positive; [|eassumption].
+  simpl. intros; tauto.
+Qed.
+
+Ltac prove_ind3 :=
+  unfold is_ind3;
+  match goal with [ |- ?G1_ /\ ?G2_ /\ ?G3_ ] =>
+    pose (G1 := G1_);
+    pose (Hmap := (ltac:(intros Q R H x y z Hxyz; destruct Hxyz; constructor; try assumption; apply H; assumption) : G1));
+    split; [exact Hmap|];
+    split; [|intros x y z Hxyz; constructor; assumption];
+    intros Q HQ; fix H 4; intros x y z Hxyz;
+    destruct Hxyz as [x1 y1 z1 Hxyz];
+    apply (Hmap _ Q) in Hxyz; [apply HQ; assumption|assumption]
+  end.
+
+End Ind3.
+
+
+Section Ind4.
+
+Context {A : Type}.
+Context {B : A -> Type}.
+Context {C : forall x, B x -> Type}.
+Context {D : forall x y, C x y -> Type}.
+Context (G : (forall x y z, D x y z -> Prop) -> (forall x y z, D x y z -> Prop)).
+Context (P : forall x y z, D x y z -> Prop).
+
+Implicit Types Q R : forall x y z, D x y z -> Prop.
+
+Definition is_ind4 :=
+  (forall Q R, (forall x y z u, Q x y z u -> R x y z u) -> forall x y z u, G Q x y z u -> G R x y z u) /\
+  (forall Q, (forall x y z u, G Q x y z u -> Q x y z u) -> forall x y z u, P x y z u -> Q x y z u) /\
+  (forall x y z u, G P x y z u -> P x y z u).
+
+Hypothesis Hind : is_ind4.
+
+Let is_positive := proj1 Hind.
+Let has_ind := proj1 (proj2 Hind).
+Let is_ind := proj2 (proj2 Hind).
+
+Definition preserved4 Q :=
+  forall x y z u, G (fun x y z u => P x y z u /\ Q x y z u) x y z u -> Q x y z u.
+Definition preserved_with_inv4 Q R :=
+  forall x y z u, G (fun x y z u => P x y z u /\ Q x y z u /\ R x y z u) x y z u -> Q x y z u.
+Definition preserved_down4 Q :=
+  forall x y z u R, G (fun x y z u => P x y z u /\ R x y z u) x y z u -> Q x y z u -> G (fun x y z u => P x y z u /\ Q x y z u /\ R x y z u) x y z u.
+
+Lemma preserved4_rec :
+  forall Q, preserved4 Q -> forall x y z u, P x y z u -> Q x y z u.
+Proof.
+  intros Q HQ.
+  enough (H : forall x y z u, P x y z u -> P x y z u /\ Q x y z u) by (intros; apply H; assumption).
+  apply has_ind. intros; split.
+  - eapply is_ind, is_positive; [|eassumption].
+    simpl. intros; tauto.
+  - apply HQ. assumption.
+Qed.
+
+Lemma preserved_with_inv4_rec :
+  forall Q R, preserved_down4 R -> preserved_with_inv4 Q R -> forall x y z u, P x y z u -> R x y z u -> Q x y z u.
+Proof.
+  intros Q R H1 H2. refine (preserved4_rec (fun x y z u => R x y z u -> Q x y z u) _).
+  intros x y z u H3 H4. apply H2.
+  apply is_positive with (Q := fun x y z u => P x y z u /\ R x y z u /\ (R x y z u -> Q x y z u)); [intros; tauto|].
+  apply H1; assumption.
+Qed.
+
+Lemma ind4_inv :
+  forall x y z u, P x y z u -> G P x y z u.
+Proof.
+  apply preserved4_rec. intros x y z u H.
+  eapply is_positive; [|eassumption].
+  simpl. intros; tauto.
+Qed.
+
+Ltac prove_ind4 :=
+  unfold is_ind4;
+  match goal with [ |- ?G1_ /\ ?G2_ /\ ?G3_ ] =>
+    pose (G1 := G1_);
+    pose (Hmap := (ltac:(intros Q R H x y z u Hxyzu; destruct Hxyzu; constructor; try assumption; apply H; assumption) : G1));
+    split; [exact Hmap|];
+    split; [|intros x y z u Hxyzu; constructor; assumption];
+    intros Q HQ; fix H 5; intros x y z u Hxyzu;
+    destruct Hxyzu as [x1 y1 z1 u1 Hxyzu];
+    apply (Hmap _ Q) in Hxyzu; [apply HQ; assumption|assumption]
+  end.
+
+End Ind4.
+
+
+Section Ind5.
+
+Context {A : Type}.
+Context {B : A -> Type}.
+Context {C : forall x, B x -> Type}.
+Context {D : forall x y, C x y -> Type}.
+Context {E : forall x y z, D x y z -> Type}.
+Context (G : (forall x y z u, E x y z u -> Prop) -> (forall x y z u, E x y z u -> Prop)).
+Context (P : forall x y z u, E x y z u -> Prop).
+
+Implicit Types Q R : forall x y z u, E x y z u -> Prop.
+
+Definition is_ind5 :=
+  (forall Q R, (forall x y z u v, Q x y z u v -> R x y z u v) -> forall x y z u v, G Q x y z u v -> G R x y z u v) /\
+  (forall Q, (forall x y z u v, G Q x y z u v -> Q x y z u v) -> forall x y z u v, P x y z u v -> Q x y z u v) /\
+  (forall x y z u v, G P x y z u v -> P x y z u v).
+
+Hypothesis Hind : is_ind5.
+
+Let is_positive := proj1 Hind.
+Let has_ind := proj1 (proj2 Hind).
+Let is_ind := proj2 (proj2 Hind).
+
+Definition preserved5 Q :=
+  forall x y z u v, G (fun x y z u v => P x y z u v /\ Q x y z u v) x y z u v -> Q x y z u v.
+Definition preserved_with_inv5 Q R :=
+  forall x y z u v, G (fun x y z u v => P x y z u v /\ Q x y z u v /\ R x y z u v) x y z u v -> Q x y z u v.
+Definition preserved_down5 Q :=
+  forall x y z u v R, G (fun x y z u v => P x y z u v /\ R x y z u v) x y z u v -> Q x y z u v -> G (fun x y z u v => P x y z u v /\ Q x y z u v /\ R x y z u v) x y z u v.
+
+Lemma preserved5_rec :
+  forall Q, preserved5 Q -> forall x y z u v, P x y z u v -> Q x y z u v.
+Proof.
+  intros Q HQ.
+  enough (H : forall x y z u v, P x y z u v -> P x y z u v /\ Q x y z u v) by (intros; apply H; assumption).
+  apply has_ind. intros; split.
+  - eapply is_ind, is_positive; [|eassumption].
+    simpl. intros; tauto.
+  - apply HQ. assumption.
+Qed.
+
+Lemma preserved_with_inv5_rec :
+  forall Q R, preserved_down5 R -> preserved_with_inv5 Q R -> forall x y z u v, P x y z u v -> R x y z u v -> Q x y z u v.
+Proof.
+  intros Q R H1 H2. refine (preserved5_rec (fun x y z u v => R x y z u v -> Q x y z u v) _).
+  intros x y z u v H3 H4. apply H2.
+  apply is_positive with (Q := fun x y z u v => P x y z u v /\ R x y z u v /\ (R x y z u v -> Q x y z u v)); [intros; tauto|].
+  apply H1; assumption.
+Qed.
+
+Lemma ind5_inv :
+  forall x y z u v, P x y z u v -> G P x y z u v.
+Proof.
+  apply preserved5_rec. intros x y z u v H.
+  eapply is_positive; [|eassumption].
+  simpl. intros; tauto.
+Qed.
+
+Ltac prove_ind5 :=
+  unfold is_ind5;
+  match goal with [ |- ?G1_ /\ ?G2_ /\ ?G3_ ] =>
+    pose (G1 := G1_);
+    pose (Hmap := (ltac:(intros Q R H x y z u v Hxyzuv; destruct Hxyzuv; constructor; try assumption; apply H; assumption) : G1));
+    split; [exact Hmap|];
+    split; [|intros x y z u v Hxyzuv; constructor; assumption];
+    intros Q HQ; fix H 6; intros x y z u v Hxyzuv;
+    destruct Hxyzuv as [x1 y1 z1 u1 v1 Hxyzuv];
+    apply (Hmap _ Q) in Hxyzuv; [apply HQ; assumption|assumption]
+  end.
+
+End Ind5.
+
+
+Section Ind6.
+
+Context {A : Type}.
+Context {B : A -> Type}.
+Context {C : forall x, B x -> Type}.
+Context {D : forall x y, C x y -> Type}.
+Context {E : forall x y z, D x y z -> Type}.
+Context {F : forall x y z u, E x y z u -> Type}.
+Context (G : (forall x y z u v, F x y z u v -> Prop) -> (forall x y z u v, F x y z u v -> Prop)).
+Context (P : forall x y z u v, F x y z u v -> Prop).
+
+Implicit Types Q R : forall x y z u v, F x y z u v -> Prop.
+
+Definition is_ind6 :=
+  (forall Q R, (forall x y z u v w, Q x y z u v w -> R x y z u v w) -> forall x y z u v w, G Q x y z u v w -> G R x y z u v w) /\
+  (forall Q, (forall x y z u v w, G Q x y z u v w -> Q x y z u v w) -> forall x y z u v w, P x y z u v w -> Q x y z u v w) /\
+  (forall x y z u v w, G P x y z u v w -> P x y z u v w).
+
+Hypothesis Hind : is_ind6.
+
+Let is_positive := proj1 Hind.
+Let has_ind := proj1 (proj2 Hind).
+Let is_ind := proj2 (proj2 Hind).
+
+Definition preserved6 Q :=
+  forall x y z u v w, G (fun x y z u v w => P x y z u v w /\ Q x y z u v w) x y z u v w -> Q x y z u v w.
+Definition preserved_with_inv6 Q R :=
+  forall x y z u v w, G (fun x y z u v w => P x y z u v w /\ Q x y z u v w /\ R x y z u v w) x y z u v w -> Q x y z u v w.
+Definition preserved_down6 Q :=
+  forall x y z u v w R, G (fun x y z u v w => P x y z u v w /\ R x y z u v w) x y z u v w -> Q x y z u v w -> G (fun x y z u v w => P x y z u v w /\ Q x y z u v w /\ R x y z u v w) x y z u v w.
+
+Lemma preserved6_rec :
+  forall Q, preserved6 Q -> forall x y z u v w, P x y z u v w -> Q x y z u v w.
+Proof.
+  intros Q HQ.
+  enough (H : forall x y z u v w, P x y z u v w -> P x y z u v w /\ Q x y z u v w) by (intros; apply H; assumption).
+  apply has_ind. intros; split.
+  - eapply is_ind, is_positive; [|eassumption].
+    simpl. intros; tauto.
+  - apply HQ. assumption.
+Qed.
+
+Lemma preserved_with_inv6_rec :
+  forall Q R, preserved_down6 R -> preserved_with_inv6 Q R -> forall x y z u v w, P x y z u v w -> R x y z u v w -> Q x y z u v w.
+Proof.
+  intros Q R H1 H2. refine (preserved6_rec (fun x y z u v w => R x y z u v w -> Q x y z u v w) _).
+  intros x y z u v w H3 H4. apply H2.
+  apply is_positive with (Q := fun x y z u v w => P x y z u v w /\ R x y z u v w /\ (R x y z u v w -> Q x y z u v w)); [intros; tauto|].
+  apply H1; assumption.
+Qed.
+
+Lemma ind6_inv :
+  forall x y z u v w, P x y z u v w -> G P x y z u v w.
+Proof.
+  apply preserved6_rec. intros x y z u v w H.
+  eapply is_positive; [|eassumption].
+  simpl. intros; tauto.
+Qed.
+
+Ltac prove_ind6 :=
+  unfold is_ind6;
+  match goal with [ |- ?G1_ /\ ?G2_ /\ ?G3_ ] =>
+    pose (G1 := G1_);
+    pose (Hmap := (ltac:(intros Q R H x y z u v w Hxyzuvw; destruct Hxyzuvw; constructor; try assumption; apply H; assumption) : G1));
+    split; [exact Hmap|];
+    split; [|intros x y z u v w Hxyzuvw; constructor; assumption];
+    intros Q HQ; fix H 7; intros x y z u v w Hxyzuvw;
+    destruct Hxyzuvw as [x1 y1 z1 u1 v1 w1 Hxyzuvw];
+    apply (Hmap _ Q) in Hxyzuvw; [apply HQ; assumption|assumption]
+  end.
+
+End Ind6.
+
+
+
+
+
+
+
+
+
+
+
+
+
+
+
+
+(*
+Inductive test (rec : nat -> nat -> Prop) : nat -> nat -> Prop :=
+| test_O : test rec O O
+| test_SS : forall n m, rec n m -> test rec (S (S n)) (S (S m)).
+
+Inductive t : nat -> nat -> Prop :=
+| t_intro : forall n m, test t n m -> t n m.
+
+Ltac prove_ind2 :=
+  unfold is_ind2;
+  match goal with [ |- ?G1_ /\ ?G2_ /\ ?G3_ ] =>
+    pose (G1 := G1_);
+    pose (Hmap := (ltac:(intros Q R H x y Hxy; destruct Hxy; constructor; try assumption; apply H; assumption) : G1));
+    split; [exact Hmap|];
+    split; [|intros x y Hxy; constructor; assumption];
+    intros Q HQ; fix H 3; intros x y Hxy;
+    destruct Hxy as [x1 y1 Hxy];
+    apply (Hmap _ Q) in Hxy; [apply HQ; assumption|assumption]
+  end.
+
+Lemma t_ind2 : is_ind2 test t.
+Proof. prove_ind2. Qed.
+
+Lemma test_preserved_down :
+  preserved_down2 test t (fun k1 k2 => k1 = k2).
+Proof.
+  intros n m X H1 H2. inversion H1; subst; constructor.
+  split; [|split]; try tauto. congruence.
+Qed.
+
+Lemma h : forall n1 n2, t n1 -> t n2 -> t (n1 + n2).
+Proof.
+  intros n1 n2 H1 H2. revert n1 H1; apply preserved_rec.
+  intros n1 Hn1. destruct Hn1.
+  - assumption.
+  - simpl. constructor. constructor. tauto.
+Qed.
+*)
